# Idempotent functions

## 题目描述

Some time ago Leonid have known about idempotent functions. Idempotent function defined on a set $ {1,2,...,n} $ is such function ![](https://cdn.luogu.com.cn/upload/vjudge_pic/CF542C/bd89689373264189cd84dae0d69467be68ca323b.png), that for any ![](https://cdn.luogu.com.cn/upload/vjudge_pic/CF542C/9a41c8470dbaa5967772aedda0040717aaf30fea.png) the formula $ g(g(x))=g(x) $ holds.

Let's denote as $ f^{(k)}(x) $ the function $ f $ applied $ k $ times to the value $ x $ . More formally, $ f^{(1)}(x)=f(x) $ , $ f^{(k)}(x)=f(f^{(k-1)}(x)) $ for each $ k&gt;1 $ .

You are given some function ![](https://cdn.luogu.com.cn/upload/vjudge_pic/CF542C/7ed3c9bd96ebefaf9c2ae2aa09921c0d35366e17.png). Your task is to find minimum positive integer $ k $ such that function $ f^{(k)}(x) $ is idempotent.

## 输入输出格式

### 输入格式

In the first line of the input there is a single integer $ n $ ( $ 1<=n<=200 $ ) — the size of function $ f $ domain.

In the second line follow $ f(1),f(2),...,f(n) $ ( $ 1<=f(i)<=n $ for each $ 1<=i<=n $ ), the values of a function.

### 输出格式

Output minimum $ k $ such that function $ f^{(k)}(x) $ is idempotent.

## 输入输出样例

### 输入样例 #1

```cpp
4
1 2 2 4

```
### 输出样例 #1

```cpp
1

```
### 输入样例 #2

```cpp
3
2 3 3

```
### 输出样例 #2

```cpp
2

```
### 输入样例 #3

```cpp
3
2 3 1

```
### 输出样例 #3

```cpp
3

```
## 说明

In the first sample test function $ f(x)=f^{(1)}(x) $ is already idempotent since $ f(f(1))=f(1)=1 $ , $ f(f(2))=f(2)=2 $ , $ f(f(3))=f(3)=2 $ , $ f(f(4))=f(4)=4 $ .

In the second sample test:

- function $ f(x)=f^{(1)}(x) $ isn't idempotent because $ f(f(1))=3 $ but $ f(1)=2 $ ;

- function $ f(x)=f^{(2)}(x) $ is idempotent since for any $ x $ it is true that $ f^{(2)}(x)=3 $ , so it is also true that $ f^{(2)}(f^{(2)}(x))=3 $ .

In the third sample test:

- function $ f(x)=f^{(1)}(x) $ isn't idempotent because $ f(f(1))=3 $ but $ f(1)=2 $ ;

- function $ f(f(x))=f^{(2)}(x) $ isn't idempotent because $ f^{(2)}(f^{(2)}(1))=2 $ but $ f^{(2)}(1)=3 $ ;

- function $ f(f(f(x)))=f^{(3)}(x) $ is idempotent since it is identity function: $ f^{(3)}(x)=x $ for any ![](https://cdn.luogu.com.cn/upload/vjudge_pic/CF542C/11e22b0eed3b852ef44d62d2479b42e2534a18a6.png) meaning that the formula $ f^{(3)}(f^{(3)}(x))=f^{(3)}(x) $ also holds.

